src/temporal_logic/basic.lean
@@ -17,103 +17,10 @@ open interactive lean.parser tactic
 open list (hiding map) has_map predicate
 local postfix *:9001 := many
 
--- meta def apply_left (r : parse texpr) : tactic unit :=
--- transitivity none ; [apply r >> done, skip]
-
--- meta def apply_right (r : parse texpr) : tactic unit :=
--- transitivity none ; [skip, apply r >> done]
-
--- meta def references_to (v : expr) : tactic (list expr) :=
--- do ctx ← local_context,
---    ctx_t ← mmap infer_type ctx,
---    return $ map prod.fst $ filter ((λ t, v.occurs t) ∘ prod.snd) $ zip ctx ctx_t
-
--- -- meta def focus_rhs (tac : itactic) : tactic unit :=
--- -- do `(_ ⟹ %%p) ← target <|> fail "expecting goal: _ ⟹ _",
--- --    t ← infer_type p,
--- --    q ← mk_meta_var t,
--- --    e ← to_expr ``(%%q ⟹ %%p),
--- --    h ← assert `h _, _
-
--- meta def mk_local_hyp (a' : expr) (hyp : pexpr) : tactic (expr × expr × expr) :=
--- do e' ← to_expr hyp,
---    e ← if e'.is_local_constant
---        then return e'
---        else note `h none e',
---    (expr.app f a)  ← infer_type e,
---    is_def_eq a a' <|> fail format!"{a} and {a'} are not the same argument",
---    return (e, f, a)
-
--- meta def revert_pred (a : expr) (h : expr × expr × expr) : tactic unit :=
--- do (expr.app g a') ← target,
---    is_def_eq a a',
---    tactic.revert h.1,
---    refine ``(impl_of_p_impl %%a _)
---    -- to_expr ``((%%h.2.1 ⟶ %%g) %%a) >>= tactic.change
-
--- meta def revert_p (hyps : parse pexpr_list_or_texpr) : tactic unit :=
--- do (expr.app g a) ← target,
---    hyps' ← mmap (mk_local_hyp a) hyps,
---    ls ← references_to a,
---    let vars := hyps'.map prod.fst,
---    mmap tactic.clear (ls.diff vars),
---    if a.is_local_constant then do -- <|> fail format!"{a} is not a local constant",
---      mmap' (revert_pred a) hyps',
---      () <$ tactic.revert a
---    else (mmap' (revert_pred a) hyps' >> tactic.generalize a),
---    -- to_expr ``(entails_of_forall_impl _) >>= infer_type >>= trace,
---    -- trace_state
---    tactic.refine ``(entails_of_forall_impl _)
---    -- to_expr ``(%%f ⟹ %%g) >>= tactic.change
-
--- private meta def apply_trans : expr → expr → list expr → tactic unit
---  | _ _ [] := return ()
---  | p q (e :: es) := refine ``(@function.comp %%p %%e %%q _ _) ; [ skip , apply_trans p e es ]
-
--- meta def imp_transitivity : parse (optional pexpr_list_or_texpr) → tactic unit
---  | none :=
--- do `(%%p → %%q) ← target <|> fail "expecting implication",
---    refine ``(@function.comp %%p _ %%q _ _) >> rotate_left 1
---  | (some xs) :=
--- do xs' ← mmap to_expr xs,
---    `(%%p → %%q) ← target <|> fail "expecting implication",
---    focus1 (apply_trans p q xs'.reverse)
-
--- meta def apply' (e : parse texpr) : tactic unit :=
--- apply e <|> (intro1 >>= λ h, (apply' ; try (tactic.exact h)) >> try (tactic.clear h))
-
 meta def TL_unfold (cs : parse ident*) (loc : parse location) : tactic unit :=
 do unfold_coes loc, unfold (cs ++ [`var.apply,`pred'.mk]) loc
 
--- meta def coes_thms : list name :=
--- [`predicate.lifted₀
--- ,`coe,`lift_t,`lift,`has_lift_t,`coe_t,`coe,`has_coe_t
--- ,`coe_b,`coe,`has_coe,`coe_fn,`coe,`has_coe_to_fun
--- ,`coe_sort,`coe,`has_coe_to_sort,`predicate.lifted₀]
-
--- -- meta def TL_simp
--- --    (only_kw : parse only_flag)
--- --    (args : parse simp_arg_list)
--- --    (w : parse with_ident_list)
--- --    (loc : parse location) : tactic unit :=
--- -- do std_lmm ← mmap (map (simp_arg_type.expr ∘ to_pexpr) ∘ mk_const) (coes_thms ++ [`predicate.var.apply,`predicate.pred'.mk,`temporal.init_to_fun]) ,
--- --    repeat (simp only_kw args w loc <|> simp only_kw std_lmm w loc <|> unfold_coes loc <|> unfold [`predicate.var.apply,`predicate.pred'.mk,`predicate.lifted₀] loc)
-
 end tactic.interactive
-
-
--- section
--- variables b : Prop
--- variables c : ℕ → Prop
--- variable h : b → ∀ i, c i
--- variable h' : ℕ
--- include h h'
--- example : ∀ i, c i :=
--- begin
---   apply h , done,
--- end
-
--- end
 
 namespace temporal
 
@@ -140,19 +47,11 @@ def henceforth (p : cpred) : cpred :=
 ⟨ λ i, ∀ j, p.apply (i+j) ⟩
 def next (p : tvar α) : tvar α :=
 ⟨ λ i, p.apply (i.succ) ⟩
--- def init (p : pred' β) : cpred :=
--- ⟨ λ τ, p.apply (τ 0) ⟩
 
--- prefix `•`:85 := init
 prefix `⊙`:90 := next
 prefix `◇`:95 := eventually -- \di
 prefix `◻`:95 := henceforth -- \sqw
--- notation `⟦`:max act `⟧`:0 := action act
 notation `⟦ `:max v ` <> `:50 R ` ⟧`:0 := action R v
--- infix ` ⊫ ` --
-  -- 216 -- notation `⦃` act `⦄`:95 := ew act
-
--- lemma init_to_fun (p : pred' β) (τ : stream β) : (•p).apply τ = p.apply (τ 0) := rfl
 
 def tl_leads_to (p q : cpred) : cpred :=
 ◻(p ⟶ ◇q)
@@ -211,18 +110,6 @@ begin
   apply h
 end
 open stream
--- lemma eventually_weaken' {p : cpred} {τ} (i) :
---   p (drop i τ) → (◇ p) τ :=
--- begin
---   intros h,
---   TL_unfold eventually,
---   existsi i,
---   apply h
--- end
-
--- lemma eventually_of_next {p : cpred}
--- : ⊙p ⟹ ◇p :=
--- sorry
 
 @[strengthening]
 lemma next_entails_eventually (p : cpred)
@@ -240,18 +127,6 @@ lemma henceforth_str (p : cpred) :
 begin
   pointwise with τ h, apply h 0
 end
-
--- lemma henceforth_str' {p : cpred} {τ} (i) :
---   (◻p) τ → p (drop i τ) :=
--- begin
---   intros h, apply h i
--- end
-
--- lemma henceforth_delay {p : cpred} {τ} (i) :
---   (◻p) τ → (◻p) (drop i τ) :=
--- begin
---   intros h j, simp [drop_drop], apply h
--- end
 
 local infix ` <$> ` := fun_app_to_var
 local infix ` <*> ` := combine_var
@@ -291,17 +166,6 @@ rfl
 lemma action_false (v : tvar α)
 : (⟦ v <> λ _ _, false ⟧ : cpred) = False :=
 by { funext x, refl }
-
--- lemma action_eq_next {p : β → β → Prop}
--- :  (⟦ p ⟧ : cpred) = (∃∃ s : β, •eq s ⋀ ⊙•p s) :=
--- begin
---   funext τ, TL_unfold action p_exists pred.p_exists,
---   split
---   ; try {TL_simp [next]}
---   ; intros
---   ; try {subst x}
---   ; assumption,
--- end
 
 variables {Γ : cpred}
 
@@ -347,14 +211,6 @@ begin
     apply h }
 end
 
--- lemma henceforth_drop {p : cpred} {τ} (i : ℕ) :
--- (◻p) τ → (◻p) (τ.drop i) :=
--- begin
---   intro h,
---   rw ← henceforth_henceforth at h,
---   apply h,
--- end
-
 /- True / False -/
 
 @[simp]
@@ -375,15 +231,6 @@ begin
   { cases h }
 end
 
--- @[simp]
--- lemma init_false : (•False) = (False : cpred) :=
--- begin
---   funext1,
---   split ; intro h,
---   { cases h },
---   { cases h }
--- end
-
 @[simp]
 lemma eventually_true : ◇(True : cpred) = True :=
 begin
@@ -392,20 +239,6 @@ begin
   { trivial },
   { apply exists.intro 0, trivial }
 end
-
--- @[simp]
--- lemma init_true : (•True) = (True : cpred) :=
--- begin
---   funext1,
---   split ; intro h ; trivial,
--- end
-
--- lemma init_exists {t} (p : t → pred' β)
--- : •(∃∃ i, p i) = ∃∃ i, •p i :=
--- begin
---   funext x,
---   TL_simp [p_exists,pred.p_exists,init]
--- end
 
 /- monotonicity -/
 
@@ -474,29 +307,13 @@ begin
   auto,
 end
 
--- @[monotonic]
--- lemma init_entails_init {p q : pred' β} (f : p ⟹ q)
--- : (•p) ⟹ (•q) :=
--- begin
---   pointwise f with i,
---   xassumption,
--- end
-
 lemma inf_often_entails_inf_often {p q : cpred} (f : p ⟹ q)
 : ◻◇p ⟹ ◻◇q :=
 by monotonicity f
 
--- lemma inf_often_entails_inf_often' {p q : pred' β} (f : p ⟹ q)
--- : ◻◇•p ⟹ ◻◇•q :=
--- by monotonicity f
-
 lemma stable_entails_stable {p q : cpred} (f : p ⟹ q)
 : ◇◻p ⟹ ◇◻q :=
 by monotonicity f
-
--- lemma stable_entails_stable' {p q : pred' β} (f : p ⟹ q)
--- : ◇◻•p ⟹ ◇◻•q :=
--- by monotonicity f
 
 lemma henceforth_and (p q : cpred)
 : ◻(p ⋀ q) = ◻p ⋀ ◻q :=
