src/temporal_logic/persistent.lean
@@ -1,0 +1,99 @@
+
+import temporal_logic.basic
+
+universe variables u u₀ u₁ u₂
+
+variables {α : Sort u₀} {β : Type u₁} {γ : Sort u₂}
+
+namespace temporal
+open predicate
+class persistent (p : cpred) : Prop :=
+  (is_persistent : ◻p = p)
+export persistent (is_persistent)
+
+instance henceforth_persistent {p : cpred} : persistent (◻p) :=
+by { constructor, simp }
+
+instance not_eventually_persistent {p : cpred} : persistent (-◇p) :=
+by { constructor, simp }
+
+instance leads_to_persistent {p q : cpred} : persistent (p ~> q) :=
+by { constructor, simp [tl_leads_to,is_persistent] }
+
+instance and_persistent {p q : cpred} [persistent p] [persistent q]
+: persistent (p ⋀ q) :=
+by { constructor, simp [henceforth_and,is_persistent], }
+
+instance true_persistent
+: persistent (True : cpred) :=
+by { constructor, simp, }
+
+instance false_persistent
+: persistent (False : cpred) :=
+by { constructor, simp, }
+
+instance forall_persistent {p : α → cpred} [∀ i, persistent (p i)]
+: persistent (p_forall p) :=
+by { constructor, simp [henceforth_forall,is_persistent], }
+
+def list_persistent (xs : list cpred) :=
+Π q ∈ xs, persistent q
+
+lemma nil_persistent
+: list_persistent [] :=
+by { intros p h, cases h }
+
+lemma cons_persistent (x : cpred) (xs : list $ cpred)
+  [persistent x]
+  (h : list_persistent xs)
+: list_persistent (x :: xs) :=
+by { intros p h, simp [list_persistent] at *,
+     cases h ; [ subst p, skip ] ; auto, }
+
+def with_h_asms (Γ : cpred) : Π (xs : list (cpred)) (x : cpred), Prop
+ | [] x := Γ ⊢ x
+ | (x :: xs) y := Γ ⊢ x → with_h_asms xs y
+
+lemma indirect_judgement (h p : pred' β)
+  (H : ∀ Γ, Γ ⊢ h → Γ ⊢ p)
+: h ⊢ p :=
+sorry
+
+lemma judgement_trans (p q r : pred' β)
+  (h₀ : p ⊢ q)
+  (h₁ : q ⊢ r)
+: p ⊢ r :=
+sorry
+
+lemma from_antecendent (xs : list (cpred)) (p : cpred)
+  (h : ∀ Γ, with_h_asms Γ xs p)
+: ◻ xs.foldr (⋀) True ⊢ p :=
+begin
+  apply indirect_judgement,
+  introv h', specialize h Γ,
+  induction xs with x xs,
+  { simp [with_h_asms] at h, apply h },
+  { simp [list.foldr,henceforth_and] at h',
+    apply ih_1,
+    { revert h',
+      apply p_impl_revert,
+      apply p_and_elim_right },
+    { apply h, revert h',
+      apply p_impl_revert,
+      apply p_and_entails_of_entails_left,
+      apply henceforth_str, } }
+end
+
+lemma persistent_to_henceforth {p q : cpred}
+  (h : ◻ p ⊢ q)
+: ◻ p ⊢ ◻ q :=
+sorry
+
+instance has_coe_to_fun_henceforth (Γ p q : cpred) : has_coe_to_fun (Γ ⊢ ◻(p ⟶ q)) :=
+{ F := λ _, Γ ⊢ p → Γ ⊢ q
+, coe := assume h, henceforth_str (p ⟶ q) Γ h  }
+
+instance has_coe_to_fun_leads_to (Γ p q : cpred) : has_coe_to_fun (Γ ⊢ p ~> q) :=
+temporal.has_coe_to_fun_henceforth _ _ _
+
+end temporal
