test/tactic.lean
@@ -1,0 +1,44 @@
+
+import temporal_logic
+
+open temporal predicate
+
+variable α : Type
+
+variables Γ p q r : cpred
+variables v₀ v₁ : tvar α
+variables f : pred' α
+variables h₀ : Γ ⊢ p ≡ q
+include h₀
+example : Γ ⊢ p ⋀ r ≡ q ⋀ r :=
+begin [temporal]
+  rw h₀,
+end
+
+example : Γ ⊢ p ⋀ r →  Γ ⊢ q ⋀ r :=
+assume _,
+begin [temporal]
+  rw ← h₀,
+end
+
+variables h₁ : Γ ⊢ ◻(p ≡ q)
+omit h₀
+include h₁
+example : Γ ⊢ ◻◇p ≡ ◻◇q :=
+begin [temporal]
+  rw h₁,
+end
+
+variables h₂ : Γ ⊢ ◻(v₀ ≃ v₁)
+include h₂
+example (h : Γ ⊢ ◇(◻(f ;; v₀ ≡ q) ⋀ p))
+: Γ ⊢ ◇(◻(f ;; v₁ ≡ q) ⋀ p) :=
+begin [temporal]
+  rw ← h₂,
+end
+
+example (h : Γ ⊢ ◇(◻(f ;; v₀ ≡ q) ⋀ p))
+: Γ ⊢ ◇(◻(f ;; v₁ ≡ q) ⋀ p) :=
+begin [temporal]
+  rw h₂ at h,
+end
